ML-KEM NTT proof for x86 AVX2 implementation
This change adds the implementation of ML-KEM Forward NTT
function and its HolLight proof of correctness. At this moment,
the implementation is the same as the one in mlkem-native
repository at https://github.com/pq-code-package/mlkem-native.

The new CONGBOUND_NTT_MONTMUL was implemented by @jargh.

Signed-off-by: Dusan Kostic <dkostic@protonmail.com>

benchmarks/benchmark.c
@@ -830,6 +830,8 @@ void call_sm2_montjscalarmul_alt(void) repeatfewer(10,sm2_montjscalarmul_alt(b1,
 void call_mldsa_ntt(void) repeat(mldsa_ntt((int32_t*)b0,(const int32_t*)b1))
 void call_mldsa_poly_reduce(void) repeat(mldsa_poly_reduce((int32_t*)b0))
 
+void call_mlkem_ntt(void) repeat(mlkem_ntt_x86((int16_t*)b0,(int16_t*)b1))
+
 void call_bignum_copy_row_from_table_8n__32_16(void) {}
 void call_bignum_copy_row_from_table_8n__32_32(void) {}
 void call_bignum_copy_row_from_table_16__32(void) {}
@@ -838,7 +840,6 @@ void call_bignum_copy_row_from_table_32__32(void) {}
 void call_bignum_emontredc_8n_cdiff__32(void) {}
 void call_mlkem_intt(void) {}
 void call_mlkem_mulcache_compute(void) {}
-void call_mlkem_ntt(void) {}
 void call_mlkem_tobytes(void) {}
 void call_mlkem_tomont(void) {}
 void call_mlkem_rej_uniform(void) {}
@@ -1529,7 +1530,7 @@ int main(int argc, char *argv[])
   timingtest(all,"mlkem_basemul_k4",call_mlkem_basemul_k4);
   timingtest(arm,"mlkem_intt",call_mlkem_intt);
   timingtest(arm,"mlkem_mulcache_compute",call_mlkem_mulcache_compute);
-  timingtest(arm,"mlkem_ntt",call_mlkem_ntt);
+  timingtest(all,"mlkem_ntt",call_mlkem_ntt);
   timingtest(all,"mlkem_reduce",call_mlkem_reduce);
   timingtest(arm,"mlkem_tobytes",call_mlkem_tobytes);
   timingtest(arm,"mlkem_tomont",call_mlkem_tomont);
